{
 "cells": [
  {
   "cell_type": "markdown",
   "metadata": {},
   "source": [
    "# 1. Introduction"
   ]
  },
  {
   "cell_type": "code",
   "execution_count": null,
   "metadata": {},
   "outputs": [],
   "source": [
    "import numpy as np\n",
    "import matplotlib.pyplot as plt\n",
    "\n",
    "%matplotlib inline"
   ]
  },
  {
   "cell_type": "markdown",
   "metadata": {},
   "source": [
    "1.\n",
    "\n",
    "$$\n",
    "\t\\begin{align*}\n",
    "\t\ty(x_n, \\pmb{w}) &= \\sum_{j=0}^M w_j x_n^j \\\\\n",
    "\t\tE(\\pmb{w}) &= \\frac{1}{2}\\sum_{n=1}^N(y(x_n, \\pmb{w})-t_n)^2 \\\\\n",
    "\t\t\t       &= \\frac{1}{2}\\sum_{n=1}^N\\left(\\sum_{j=0}^M w_j x_n^j-t_n\\right)^2 \\\\\n",
    "\t\\end{align*}\n",
    "$$\n",
    "Differentiating with respect to $w_i$,\n",
    "$$\n",
    "\t\\begin{align*}\n",
    "\t\t\\frac{\\mathrm{d}E(\\pmb{w})}{\\mathrm{d}w_i} &= \\sum_{n=1}^N\\left(\\sum_{j=0}^M w_j x_n^j-t_n\\right)x_n^i \\\\\n",
    "\t\t&= \\sum_{n=1}^N\\sum_{j=0}^M w_j x_n^{i+j}-\\sum_{n=1}^N t_n x_n^i \\\\\n",
    "\t\t&= \\sum_{j=0}^M\\left(\\sum_{n=1}^N x_n^{i+j}\\right) w_j-\\sum_{n=1}^N t_n x_n^i \\\\\n",
    "\t\\end{align*}\n",
    "$$\n",
    "Setting this derivative to 0 we get,\n",
    "$$\n",
    "\t\\begin{align*}\n",
    "\t\t\\sum_{j=0}^M\\left(\\sum_{n=1}^N x_n^{i+j}\\right) w_j-\\sum_{n=1}^N t_n x_n^i &= 0 \\\\\n",
    "\t\t\\implies \\sum_{j=0}^M\\left(\\sum_{n=1}^N x_n^{i+j}\\right) w_j &= \\sum_{n=1}^N t_n x_n^i \\\\\n",
    "\t\t\\implies \\sum_{j=0}^M A_{ij} w_j &= T_i\\\\\n",
    "\t\\end{align*}\n",
    "$$\n",
    "where\n",
    "$$\n",
    "    \\begin{align*}\n",
    "        A_{ij} = \\sum_{n=1}^N (x_n)^{i+j} & & T_i = \\sum_{n=1}^N (x_n)^i t_n\n",
    "    \\end{align*}\n",
    "$$\n",
    "This is a linear equation for each $i \\in \\{0, 1, \\dots, n\\}$ which together form a system of linear equations. This can be written in matrix form as\n",
    "$$\n",
    "    \\begin{align*}\n",
    "        A\\pmb{w} = T\n",
    "    \\end{align*}\n",
    "$$"
   ]
  },
  {
   "cell_type": "markdown",
   "metadata": {},
   "source": [
    "2.\n",
    "\n",
    "$$\n",
    "\t\\begin{align*}\n",
    "\t\ty(x_n, \\pmb{w}) &= \\sum_{j=0}^M w_j x_n^j \\\\\n",
    "\t\tE(\\pmb{w}) &= \\frac{1}{2}\\sum_{n=1}^N(y(x_n, \\pmb{w})-t_n)^2 + \\frac{\\lambda}{2}\\|\\pmb{w}\\|^2\\\\\n",
    "\t\t\t       &= \\frac{1}{2}\\sum_{n=1}^N\\left(\\sum_{j=0}^M w_j x_n^j-t_n\\right)^2 + \\frac{\\lambda}{2}\\sum_{j=0}^M w_j^2\\\\\n",
    "\t\\end{align*}\n",
    "$$\n",
    "Differentiating with respect to $w_i$,\n",
    "$$\n",
    "\\begin{align*}\n",
    "\t\t\\frac{\\mathrm{d}E(\\pmb{w})}{\\mathrm{d}w_i} &= \\sum_{n=1}^N\\left(\\sum_{j=0}^M w_j x_n^j-t_n\\right)x_n^i + \\lambda w_i\\\\\n",
    "\t\t&= \\sum_{n=1}^N\\sum_{j=0}^M w_j x_n^{i+j}-\\sum_{n=1}^N t_n x_n^i + \\lambda w_i \\\\\n",
    "\t\t&= \\sum_{j=0}^M\\left(\\lambda\\delta_{ij} + \\sum_{n=1}^N x_n^{i+j}\\right) w_j-\\sum_{n=1}^N t_n x_n^i \\\\\n",
    "\t\\end{align*}\n",
    "$$\n",
    "Setting this derivative to 0 we get,\n",
    "$$\n",
    "\\begin{align*}\n",
    "\t\t\\sum_{j=0}^M\\left(\\lambda\\delta_{ij} + \\sum_{n=1}^N x_n^{i+j}\\right) w_j-\\sum_{n=1}^N t_n x_n^i &= 0 \\\\\n",
    "\t\t\\implies \\sum_{j=0}^M\\left(\\lambda\\delta_{ij} + \\sum_{n=1}^N x_n^{i+j}\\right) w_j &= \\sum_{n=1}^N t_n x_n^i \\\\\n",
    "\t\t\\implies \\sum_{j=0}^M (\\lambda\\delta_{ij} + A_{ij}) w_j &= T_i\\\\\n",
    "\t\\end{align*}\n",
    "$$\n",
    "where\n",
    "$$\n",
    "    \\begin{align*}\n",
    "        A_{ij} = \\sum_{n=1}^N (x_n)^{i+j} & & T_i = \\sum_{n=1}^N (x_n)^i t_n\n",
    "    \\end{align*}\n",
    "$$\n",
    "This is a linear equation for each $i \\in \\{0, 1, \\dots, n\\}$ which together form a system of linear equations. This can be written in matrix form as\n",
    "$$\n",
    "    \\begin{align*}\n",
    "        (A + \\lambda I_n)\\pmb{w} = T\n",
    "    \\end{align*}\n",
    "$$\n",
    "where $I_n$ is the $n\\times n$ identity matrix."
   ]
  },
  {
   "cell_type": "markdown",
   "metadata": {},
   "source": [
    "3.\n",
    "\n",
    "$$\n",
    "\t\\begin{align*}\n",
    "\t\tp(a) &= p(a, r) + p(a, b) + p(a, g) \\\\\n",
    "\t\t     &= p(r)p(a | r) + p(b)p(a | b) + p(g)p(a | g) \\\\\n",
    "\t\t     &= 0.2 \\times 3/10 + 0.2 \\times 1/2 + 0.6 \\times 3/10 \\\\\n",
    "\t\t     &= 0.34 \\\\\n",
    "\t\tp(g|o) &= \\frac{p(g)p(o|g)}{p(o)} \\\\\n",
    "\t\t\t   &= \\frac{p(g)p(o|g)}{p(r)p(o|r) + p(b)p(o|b) + p(g)p(o|g)} \\\\\n",
    "\t\t\t   &= \\frac{0.6 \\times 3/10}{0.2 \\times 4/10 + 0.2 \\times 1/2 + 0.6 \\times 3/10} \\\\\n",
    "\t\t\t   &= 0.5\n",
    "\t\\end{align*}\n",
    "$$"
   ]
  },
  {
   "cell_type": "markdown",
   "metadata": {},
   "source": [
    "4.\n",
    "\n",
    "$$\n",
    "\t\\begin{align*}\n",
    "\t\tx &= g(y) \\\\\n",
    "\t\t\\implies p_y(y) &= p_x(g(y))|g'(y)| \\\\\n",
    "\t\\end{align*}\n",
    "$$\n",
    "Differentiating with respect to $y$,\n",
    "$$\n",
    "\t\\begin{align*}\n",
    "\t\tp_y'(y) = p_x'(g(y))g'(y)|g'(y)| + p_x(g(y))g''(y)\\frac{|g'(y)|}{g'(y)}\n",
    "\t\\end{align*}\n",
    "$$\n",
    "At the location $\\hat{y}$ of the maximum of the density in $y$, the above derivative is 0\n",
    "$$\n",
    "    \\begin{align*}\n",
    "\t\tp_y'(\\hat{y}) = p_x'(g(\\hat{y}))g'(\\hat{y})|g'(\\hat{y})| + p_x(g(\\hat{y}))g''(\\hat{y})\\frac{|g'(\\hat{y})|}{g'(\\hat{y})} &= 0 \\\\\n",
    "\t\t\\implies p_x'(g(\\hat{y}))g'(\\hat{y}) + p_x(g(\\hat{y}))\\frac{g''(\\hat{y})}{g'(\\hat{y})} &= 0 & (\\because |g'(\\hat{y})| \\neq 0 \\text{ in general}) \\\\\n",
    "\t\\end{align*}\n",
    "$$\n",
    "If the location $\\hat{x}$ of the maximum of the density in $x$ were such that $\\hat{x} = g(\\hat{y})$ then the above equation will reduce to\n",
    "$$\n",
    "    \\begin{align*}\n",
    "\t\tp_x'(\\hat{x})g'(\\hat{y}) + p_x(\\hat{x})\\frac{g''(\\hat{y})}{g'(\\hat{y})} &= 0 \\\\\n",
    "\t\t\\implies p_x(\\hat{x})\\frac{g''(\\hat{y})}{g'(\\hat{y})} &= 0 & (\\because p_x'(\\hat{x}) = 0)\n",
    "\t\\end{align*}\n",
    "$$\n",
    "But the last equation is not true in general (for example consider $y \\sim \\mathcal{N}(1, 1), \\ x = y^2$).\n",
    "\n",
    "If the transformation is linear, i.e., $x = ay, a \\neq 0$, we have,\n",
    "$$\n",
    "    \\begin{align*}\n",
    "\t\tp_y(y) &= p_x(ay)|a| \\\\\n",
    "\t\\end{align*}\n",
    "$$\n",
    "Differentiating with respect to $y$,\n",
    "$$\n",
    "    \\begin{align*}\n",
    "\t\tp_y'(y) &= p_x'(ay)a|a| \\\\\n",
    "\t\\end{align*}\n",
    "$$\n",
    "At $\\hat{y}$,\n",
    "$$\n",
    "    \\begin{align*}\n",
    "\t\t0 = p_y'(\\hat{y}) = p_x'(a\\hat{y})a|a| \\\\\n",
    "\t\t\\implies p_x'(a\\hat{y}) = 0 \\implies \\hat{x} = a\\hat{y} = g(\\hat{y})\n",
    "\t\\end{align*}\n",
    "$$\n",
    "Note that this is trivially true even for the case $a=0$."
   ]
  },
  {
   "cell_type": "markdown",
   "metadata": {},
   "source": [
    "5.\n",
    "\n",
    "$$\n",
    "\t\\begin{align*}\n",
    "\t\t\\mathrm{var}[f(x)] &= \\mathbb{E}[(f(x) - \\mathbb{E}[f(x)])^2] \\\\\n",
    "\t\t\t\t\t\t   &= \\mathbb{E}[f(x)^2 - 2f(x)\\mathbb{E}[f(x)] + \\mathbb{E}[f(x)]^2] \\\\\n",
    "\t\t\t\t\t\t   &= \\mathbb{E}[f(x)^2] - 2\\mathbb{E}[f(x)\\mathbb{E}[f(x)]] + \\mathbb{E}[\\mathbb{E}[f(x)]^2] \\\\\n",
    "\t\t\t\t\t\t   &= \\mathbb{E}[f(x)^2] - 2\\mathbb{E}[f(x)]^2 + \\mathbb{E}[f(x)]^2 \\\\\n",
    "\t\t\t\t\t\t   &= \\mathbb{E}[f(x)^2] - \\mathbb{E}[f(x)]^2 \\\\\n",
    "\t\\end{align*}\n",
    "$$"
   ]
  },
  {
   "cell_type": "markdown",
   "metadata": {},
   "source": [
    "6.\n",
    "\n",
    "$$\n",
    "\t\\begin{align*}\n",
    "\t\t\\mathbb{E}_{x,y}[xy] = \\int xy p(x, y) \\mathrm{d}x \\mathrm{d}y\n",
    "\t\\end{align*}\n",
    "$$\n",
    "If $x, y$ are independent, $p(x, y) = p(x)p(y)$. So, the above expectation becomes\n",
    "$$\n",
    "    \\begin{align*}\n",
    "\t\t\\mathbb{E}_{x,y}[xy] &= \\int xy p(x)p(y) \\mathrm{d}x \\mathrm{d}y \\\\\n",
    "\t\t\t\t\t\t\t &= \\int x p(x) \\mathrm{d}x \\int yp(y) \\mathrm{d}y \\\\\n",
    "\t\t\t\t\t\t\t &= \\mathbb{E}[x]\\mathbb{E}[y]\n",
    "\t\\end{align*}\n",
    "$$\t\n",
    "So when $x,y$ are independent $\\mathrm{cov}[x,y] = \\mathbb{E}_{x,y}[xy] - \\mathbb{E}[x]\\mathbb{E}[y] = \\mathbb{E}[x]\\mathbb{E}[y] - \\mathbb{E}[x]\\mathbb{E}[y] = 0$\n",
    "\n",
    "We can show that $\\mathbb{E}_{x,y}[xy] = \\mathbb{E}[x]\\mathbb{E}[y]$ even when $x, y$ are independent discrete random variables."
   ]
  },
  {
   "cell_type": "markdown",
   "metadata": {},
   "source": [
    "7.\n",
    "\n",
    "$$\n",
    "\t\\begin{align*}\n",
    "\t\tI &= \\int_{-\\infty}^{\\infty} \\exp{\\left(-\\frac{1}{2\\sigma^2}x^2\\right)}\\mathrm{d}x \\\\\n",
    "\t\tI^2 &= \\int_{-\\infty}^{\\infty} \\int_{-\\infty}^{\\infty} \\exp{\\left(-\\frac{1}{2\\sigma^2}x^2 - \\frac{1}{2\\sigma^2}y^2\\right)} \\, \\mathrm{d}x \\, \\mathrm{d}y \\\\\n",
    "\t\\end{align*}\n",
    "$$\n",
    "Transforming to polar coordinates,\n",
    "$$\n",
    "    \\begin{align*}\n",
    "\t\tI^2 &= \\int_{0}^{2\\pi} \\int_{0}^{\\infty} \\exp{\\left(-\\frac{1}{2\\sigma^2}r^2\\right)} \\, r\\mathrm{d}r \\, \\mathrm{d}\\theta \\\\\n",
    "\t\t    &= \\int_{0}^{\\infty} \\exp{\\left(-\\frac{1}{2\\sigma^2}r^2\\right)} \\, r\\mathrm{d}r \\int_{0}^{2\\pi} \\, \\mathrm{d}\\theta \\\\\n",
    "\t\t    &= 2\\pi\\int_{0}^{\\infty} \\exp{\\left(-\\frac{1}{2\\sigma^2}r^2\\right)} \\, r\\mathrm{d}r \\\\\n",
    "\t\\end{align*}\n",
    "$$\n",
    "Substituting $u = r^2$ we get,\n",
    "$$\n",
    "    \\begin{align*}\n",
    "\t\tI^2 &= 2\\pi\\int_{0}^{\\infty} \\exp{\\left(-\\frac{1}{2\\sigma^2}u\\right)} \\, \\frac{1}{2} \\mathrm{d}u \\\\\n",
    "\t\t\t&= \\pi\\int_{0}^{\\infty} \\exp{\\left(-\\frac{1}{2\\sigma^2}u\\right)} \\, \\mathrm{d}u \\\\\n",
    "\t\t\t&= 2\\pi\\sigma^2 \\\\\n",
    "\t\t\t\\implies I &= (2\\pi\\sigma^2)^{1/2}\n",
    "\t\\end{align*}\n",
    "$$\n",
    "Let's now verify the normalization condition for the Gaussian distribution,\n",
    "$$\n",
    "    \\begin{align*}\n",
    "\t\t\\int_{-\\infty}^{\\infty}\\mathcal{N}(x|\\mu,\\sigma^2) \\, \\mathrm{d}x &= \\int_{-\\infty}^{\\infty}\\frac{1}{(2\\pi\\sigma^2)^{1/2}}\\exp{\\left(\\frac{-1}{2\\sigma^2}(x-\\mu)^2\\right)}\\, \\mathrm{d}x\n",
    "\t\\end{align*}\n",
    "$$\n",
    "Substituting $t = x - \\mu$,\n",
    "$$\n",
    "    \\begin{align*}\n",
    "\t\t\\int_{-\\infty}^{\\infty}\\mathcal{N}(x|\\mu,\\sigma^2) \\, \\mathrm{d}x &= \\int_{-\\infty}^{\\infty}\\frac{1}{(2\\pi\\sigma^2)^{1/2}}\\exp{\\left(\\frac{-1}{2\\sigma^2}t^2\\right)}\\, \\mathrm{d}t \\\\\n",
    "\t\t&= \\frac{1}{(2\\pi\\sigma^2)^{1/2}} \\int_{-\\infty}^{\\infty}\\exp{\\left(\\frac{-1}{2\\sigma^2}t^2\\right)}\\, \\mathrm{d}t \\\\\n",
    "\t\t&= \\frac{1}{(2\\pi\\sigma^2)^{1/2}} I = 1\n",
    "\t\\end{align*}\n",
    "$$"
   ]
  },
  {
   "cell_type": "markdown",
   "metadata": {},
   "source": [
    "11.\n",
    "\n",
    "$$\n",
    "\t\\begin{align*}\n",
    "\t\t\\ln p(\\pmb{x}|\\mu, \\sigma^2) = -\\frac{1}{2\\sigma^2}\\sum_{n=1}^{N}(x_n-\\mu)^2-\\frac{N}{2}\\ln \\sigma^2 - \\frac{N}{2}\\ln (2\\pi)\n",
    "\t\\end{align*}\n",
    "$$\n",
    "Differentiating log-likelihood with respect to $\\mu$,\n",
    "$$\n",
    "\t\\begin{align*}\n",
    "\t\t\\frac{\\mathrm{d}\\ln p(\\pmb{x}|\\mu, \\sigma^2)}{\\mathrm{d}\\mu} = \\frac{1}{2\\sigma^2}\\sum_{n=1}^{N}2(x_n-\\mu)\n",
    "\t\\end{align*}\n",
    "$$\n",
    "Setting it to 0, we get:\n",
    "$$\n",
    "\t\\begin{align*}\n",
    "\t\t\\sum_{n=1}^{N}(x_n-\\mu_{ML}) &= 0 \\\\\n",
    "\t\t\\implies \\mu_{ML} &= \\frac{1}{N}\\sum_{n=1}^{N}x_n\n",
    "\t\\end{align*}\n",
    "$$\n",
    "Differentiating log-likelihood with respect to $\\sigma^2$ ($\\mu$ is set to its optimal value $\\mu_{ML}$),\n",
    "$$\n",
    "\t\\begin{align*}\n",
    "\t\\frac{\\mathrm{d}\\ln p(\\pmb{x}|\\mu, \\sigma^2)}{\\mathrm{d}\\sigma^2} = \\frac{1}{2\\sigma^4}\\sum_{n=1}^{N}(x_n-\\mu_{ML})^2-\\frac{N}{2\\sigma^2}\n",
    "\t\\end{align*}\n",
    "$$\n",
    "Setting it to 0, we get:\n",
    "$$\n",
    "\t\\begin{align*}\n",
    "\t\t\\sigma_{ML}^2 = \\frac{1}{N}\\sum_{n=1}^N(x-\\mu_{ML})^2\n",
    "\t\\end{align*}\n",
    "$$"
   ]
  },
  {
   "cell_type": "markdown",
   "metadata": {},
   "source": [
    "30.\n",
    "\n",
    "$$\n",
    "\t\\begin{align*}\n",
    "\t\t\\mathrm{KL}(p\\|q) &= -\\int p(x) \\ln \\left(\\frac{q(x)}{p(x)}\\right) \\mathrm{d}x \\\\\n",
    "\t\t\t\t\t\t  &= -\\int p(x) \\ln \\left(\\frac{\\frac{1}{\\sqrt{2\\pi s^2}}e^{\\frac{-(x-m)^2}{2s^2}}}{\\frac{1}{\\sqrt{2\\pi \\sigma^2}}e^{\\frac{-(x-\\mu)^2}{2\\sigma^2}}}\\right) \\mathrm{d}x \\\\\n",
    "\t\t\t\t\t\t  &= -\\int p(x) \\left( \\ln \\left(\\frac{\\sigma}{s}\\right) + \\frac{(x-\\mu)^2}{2\\sigma^2} - \\frac{(x-m)^2}{2s^2}\\right) \\mathrm{d}x \\\\\n",
    "\t\t\t\t\t\t  &= \\ln \\frac{s}{\\sigma} + \\frac{1}{2s^2}\\mathrm{E}_p[(x-m)^2]-\\frac{1}{2\\sigma^2}\\mathrm{E}_p[(x-\\mu)^2] \\\\\n",
    "\t\t\t\t\t\t  &= \\ln \\frac{s}{\\sigma} + \\frac{1}{2s^2}(\\mu^2 + \\sigma^2 - 2m\\mu + m^2) - \\frac{1}{2} \\\\\n",
    "\t\t\t\t\t\t  &= \\ln \\frac{s}{\\sigma} + \\frac{1}{2s^2}(\\sigma^2 + (\\mu - m)^2) - \\frac{1}{2} \\\\\n",
    "\t\\end{align*}\n",
    "$$"
   ]
  },
  {
   "cell_type": "markdown",
   "metadata": {},
   "source": [
    "35.\n",
    "\n",
    "$$\n",
    "\t\\begin{align*}\n",
    "\t\tp(x) &= \\frac{1}{(2\\pi \\sigma^2)^{1/2}}e^{-\\frac{(x-\\mu)^2}{2\\sigma^2}} \\\\\n",
    "\t\t\\mathrm{H}[x] &= -\\int p(x) \\ln p(x) \\mathrm{d}x \\\\\n",
    "\t\t\t\t\t  &= -\\int p(x) \\ln \\left(\\frac{1}{(2\\pi \\sigma^2)^{1/2}}e^{-\\frac{(x-\\mu)^2}{2\\sigma^2}}\\right) \\mathrm{d}x\\\\\n",
    "\t\t\t\t\t  &= -\\int p(x) \\left(-\\frac{1}{2}\\ln (2\\pi \\sigma^2) - \\frac{(x-\\mu)^2}{2\\sigma^2}\\right) \\mathrm{d}x \\\\\n",
    "\t\t\t\t\t  &= \\frac{1}{2} \\ln (2\\pi \\sigma^2) \\int p(x) \\mathrm{d}x + \\int p(x) \\frac{(x-\\mu)^2}{2\\sigma^2} \\mathrm{d}x \\\\\n",
    "\t\t\t\t\t  &= \\frac{1}{2} \\ln (2\\pi \\sigma^2) \\times 1 + \\frac{1}{2\\sigma^2} \\times \\sigma^2 \\\\\n",
    "\t\t\t\t\t  &= \\frac{1}{2}\\left(1 + \\ln(2\\pi \\sigma^2)\\right)\n",
    "\t\\end{align*}\n",
    "$$"
   ]
  },
  {
   "cell_type": "code",
   "execution_count": null,
   "metadata": {},
   "outputs": [],
   "source": [
    "x = np.linspace(1e-6, 1, num=50)\n",
    "y = 0.5 * (1 + np.log(2 * np.pi * x))\n",
    "\n",
    "plt.plot(x, y)\n",
    "plt.title(\"Entropy of Gaussian distribution vs Variance\")\n",
    "plt.xlabel(r\"$\\sigma^2$\")\n",
    "plt.ylabel(r\"$\\mathrm{H}[X]$\")\n",
    "plt.show()"
   ]
  },
  {
   "cell_type": "markdown",
   "metadata": {},
   "source": [
    "Note that unlike in the discrete case, entropy can be negative for continuous random variables!"
   ]
  },
  {
   "cell_type": "markdown",
   "metadata": {},
   "source": [
    "40.\n",
    "\n",
    "Let $a_1, a_2, \\dots, a_n$ be $n$ real numbers. Applying Jensen's inequality (1.115) to the concave function $f(x) = \\ln x$ on $a_1, a_2, \\dots, a_n$ with $\\lambda_i = \\frac{1}{n} \\, \\forall i$ gives:\n",
    "$$\n",
    "\t\\begin{align*}\n",
    "\t\t\\ln \\left({\\frac{1}{n}\\sum_{i=1}^n a_i}\\right) &\\geq \\frac{1}{n}\\sum_{i=1}^n\\ln a_i \\\\\n",
    "\t\t\t\t\t\t\t\t\t\t\t\t\t   &\\geq \\frac{1}{n}\\ln \\prod_{i=1}^n a_i \\\\\n",
    "\t\t\t\t\t\t\t\t\t\t\t\t\t   &\\geq \\ln \\left(\\prod_{i=1}^n a_i\\right)^{\\frac{1}{n}} \\\\\n",
    "\t\t\\text{Exponentiating on both sides,} \\\\\n",
    "\t\t\\frac{1}{n}\\sum_{i=1}^n a_i &\\geq \\left(\\prod_{i=1}^n a_i\\right)^{\\frac{1}{n}}\n",
    "\t\\end{align*}\n",
    "$$"
   ]
  },
  {
   "cell_type": "markdown",
   "metadata": {},
   "source": [
    "41.\n",
    "\n",
    "$$\n",
    "\t\\begin{align*}\n",
    "\t\t\\mathrm{I}[\\pmb{x}, \\pmb{y}] &\\equiv \\mathrm{KL}(p(\\pmb{x}, \\pmb{y}) \\| p(\\pmb{x})p(\\pmb{y})) \\\\\n",
    "\t\t&= -\\int \\int p(\\pmb{x}, \\pmb{y}) \\ln {\\frac{p(\\pmb{x})p(\\pmb{y})}{p(\\pmb{x}, \\pmb{y})}} \\mathrm{d}\\pmb{x}\\mathrm{d}\\pmb{y} \\\\\n",
    "\t\t&= -\\int \\int p(\\pmb{x}, \\pmb{y}) \\ln {\\frac{p(\\pmb{x})p(\\pmb{y})}{p(\\pmb{x}) p(\\pmb{y}|\\pmb{x})}} \\mathrm{d}\\pmb{x}\\mathrm{d}\\pmb{y} \\\\\n",
    "\t\t&= -\\int \\int p(\\pmb{x}, \\pmb{y}) \\ln {\\frac{p(\\pmb{y})}{p(\\pmb{y}|\\pmb{x})}} \\mathrm{d}\\pmb{x}\\mathrm{d}\\pmb{y} \\\\\n",
    "\t\t&= -\\int \\int p(\\pmb{x}, \\pmb{y}) (\\ln {p(\\pmb{y})} - \\ln {p(\\pmb{y}|\\pmb{x})}) \\mathrm{d}\\pmb{x}\\mathrm{d}\\pmb{y} \\\\\n",
    "\t\t&= -\\int \\int p(\\pmb{x}, \\pmb{y}) \\ln {p(\\pmb{y})} \\mathrm{d}\\pmb{x}\\mathrm{d}\\pmb{y} + \\int \\int p(\\pmb{x}, \\pmb{y}) \\ln {p(\\pmb{y}|\\pmb{x})}) \\mathrm{d}\\pmb{x}\\mathrm{d}\\pmb{y} \\\\\n",
    "\t\t&= -\\int p(\\pmb{y}) \\ln {p(\\pmb{y})} \\mathrm{d}\\pmb{y} + \\int \\int p(\\pmb{x}, \\pmb{y}) \\ln {p(\\pmb{y}|\\pmb{x})}) \\mathrm{d}\\pmb{x}\\mathrm{d}\\pmb{y} \\\\\n",
    "\t\t&= \\mathrm{H}(\\pmb{y}) - \\mathrm{H}(\\pmb{y}|\\pmb{x}) \\\\\n",
    "\t\t\\text{Similarly,    } &= \\mathrm{H}(\\pmb{x}) - \\mathrm{H}(\\pmb{x}|\\pmb{y})\n",
    "\t\\end{align*}\n",
    "$$"
   ]
  }
 ],
 "metadata": {
  "kernelspec": {
   "display_name": "Python 3",
   "language": "python",
   "name": "python3"
  },
  "language_info": {
   "codemirror_mode": {
    "name": "ipython",
    "version": 3
   },
   "file_extension": ".py",
   "mimetype": "text/x-python",
   "name": "python",
   "nbconvert_exporter": "python",
   "pygments_lexer": "ipython3",
   "version": "3.6.8"
  }
 },
 "nbformat": 4,
 "nbformat_minor": 2
}
